theories/typing/cont_context.v
@@ -14,9 +14,12 @@ Section cont_context.
   }.
 
   Definition cctx_elt_interp (tid: thread_id) (c: cctx_elt) : iProp Σ :=
-    □ let 'CCtxe k L _ _ T pre := c in ∀vl vπl,
+    let 'CCtxe k L _ _ T pre := c in ∀vl vπl,
       na_own tid ⊤ -∗ llctx_interp L 1 -∗ tctx_interp tid (T vl) vπl -∗
         ⟨π, pre (vπl -$ π)⟩ -∗ WP k (map of_val vl) {{ _, cont_postcondition }}.
+
+  Definition cctx_interp (tid: thread_id) (C: list cctx_elt) : iProp Σ :=
+    ∀c, ⌜c ∈ C⌝ -∗ cctx_elt_interp tid c.
 
 End cont_context.
 Add Printing Constructor cctx_elt.
@@ -26,17 +29,36 @@ Notation cctx := (list cctx_elt).
 Notation "k ◁cont{ L , T } pre" := (CCtxe k L _ _ T pre)
   (at level 55, format "k  ◁cont{ L ,  T }  pre").
 
-Notation cctx_interp tid := (big_sepL (λ _, cctx_elt_interp tid)).
-
 Section cont_context.
   Context `{!typeG Σ}.
 
-  Lemma cctx_interp_forall tid C :
-    cctx_interp tid C ⊣⊢ ∀c, ⌜c ∈ C⌝ → cctx_elt_interp tid c.
-  Proof. by rewrite big_sepL_forall'. Qed.
-
   Global Instance cctx_interp_permut tid :
-    Proper ((≡ₚ) ==> (⊣⊢)) (cctx_interp tid) := _.
+    Proper ((≡ₚ) ==> (⊣⊢)) (cctx_interp tid).
+  Proof. solve_proper. Qed.
+
+  Lemma cctx_interp_cons tid c C :
+    cctx_interp tid (c :: C) ⊣⊢ cctx_elt_interp tid c ∧ cctx_interp tid C.
+  Proof.
+    iSplit; iIntros "cC".
+    - iSplit; [|iIntros (??)]; iApply "cC"; iPureIntro; by constructor.
+    - iIntros (? In). move: In. rewrite elem_of_cons. case=> [->|?].
+      + by iDestruct "cC" as "[? _]".
+      + iDestruct "cC" as "[_ C]". by iApply "C".
+  Qed.
+
+  Lemma cctx_interp_nil tid : cctx_interp tid [] ⊣⊢ True.
+  Proof. iSplit; [by iIntros|]. iIntros "_ % %In". inversion In. Qed.
+
+  Lemma cctx_interp_app tid C C' :
+    cctx_interp tid (C ++ C') ⊣⊢ cctx_interp tid C ∧ cctx_interp tid C'.
+  Proof.
+    elim C. { by rewrite/= cctx_interp_nil left_id. } move=>/= ?? IH.
+    by rewrite !cctx_interp_cons IH assoc.
+  Qed.
+
+  Lemma cctx_interp_singleton tid c :
+    cctx_interp tid [c] ⊣⊢ cctx_elt_interp tid c.
+  Proof. by rewrite cctx_interp_cons cctx_interp_nil right_id. Qed.
 
   Definition cctx_incl (E: elctx) (C C': cctx) : Prop :=
     ∀tid, lft_ctx -∗ proph_ctx -∗ uniq_ctx -∗
@@ -51,21 +73,21 @@ Section cont_context.
 
   Lemma incl_cctx_incl E C1 C2 : C1 ⊆ C2 → cctx_incl E C2 C1.
   Proof.
-    iIntros (Sub ?) "_ _ _ _ C". rewrite !cctx_interp_forall.
-    iIntros (? In). move/Sub in In. by iApply "C".
+    iIntros (Sub ?) "_ _ _ _ C". iIntros (? In). move/Sub in In. by iApply "C".
   Qed.
 
   Lemma cctx_incl_nil E C : cctx_incl E C [].
-  Proof. by iIntros. Qed.
+  Proof. iIntros "% _ _ _ _ _ % %In". inversion In. Qed.
 
-  Lemma cctx_incl_cons {𝔄l} k L n (T T': vec val n → tctx 𝔄l) pre tr C C' E :
+  Lemma cctx_incl_cons {𝔄l} k L n (T T': vec _ n → tctx 𝔄l) pre tr C C' E :
     cctx_incl E C C' → (∀vl, tctx_incl E L (T' vl) (T vl) tr) →
     cctx_incl E (k ◁cont{L, T} pre :: C) (k ◁cont{L, T'} (tr pre) :: C').
   Proof.
-    iIntros (InC InT ?) "#LFT #PROPH #UNIQ #E /=#[k C]".
-    iSplit; [|by iApply InC]. iIntros "!>" (??) "Na L T' Obs".
-    iMod (InT with "LFT PROPH UNIQ E L T' Obs") as (?) "(L & T & Obs)".
-    iApply ("k" with "Na L T Obs").
+    iIntros (InC InT ?) "LFT PROPH UNIQ E kC". rewrite !cctx_interp_cons. iSplit.
+    - iDestruct "kC" as "[k _]". iIntros (??) "Na L T' Obs".
+      iMod (InT with "LFT PROPH UNIQ E L T' Obs") as (?) "(L & T & Obs)".
+      iApply ("k" with "Na L T Obs").
+    - iDestruct "kC" as "[_ ?]". by iApply (InC with "LFT PROPH UNIQ E").
   Qed.
 
 End cont_context.
