theories/typing/function.v
@@ -6,13 +6,19 @@ Set Default Proof Using "Type".
 
 Implicit Type (𝔄 𝔅: syn_type) (𝔄l 𝔅l: syn_typel).
 
-Local Fixpoint subst'_pv {𝔄l} (bl: plistc binder 𝔄l) (vl: plistc val 𝔄l)
+Fixpoint subst_plv {𝔄l} (bl: plistc binder 𝔄l) (vl: plistc val 𝔄l)
   (e: expr) : expr := match 𝔄l, bl, vl with [], _, _ => e |
-    _ :: _, b -:: bl', v -:: vl' => subst' b v (subst'_pv bl' vl' e) end.
+    _ :: _, b -:: bl', v -:: vl' => subst' b v (subst_plv bl' vl' e) end.
 
-Local Lemma subst'_pv_renew {𝔄l 𝔅l} (bl: _ 𝔄l) (vl': _ 𝔅l) ew e :
-  subst'_pv (plistc_renew ew bl) vl' e =
-    subst'_pv bl (plistc_renew (symm_eq_len_wit ew) vl') e.
+Instance do_subst_plv {𝔄l} (bl vl: plistc _ 𝔄l) e :
+  DoSubstL bl (map of_val vl) e (subst_plv bl vl e).
+Proof.
+  rewrite /DoSubstL. induction 𝔄l, bl, vl; [done|]=>/=. by rewrite IH𝔄l.
+Qed.
+
+Lemma subst_plv_renew {𝔄l 𝔅l} (bl: _ 𝔄l) (vl': _ 𝔅l) ew e :
+  subst_plv (plistc_renew ew bl) vl' e =
+    subst_plv bl (plistc_renew (symm_eq_len_wit ew) vl') e.
 Proof.
   move: 𝔄l 𝔅l bl vl' ew. fix FIX 1. case=> [|??]; case=>//= ??[??][??]?.
   f_equal. apply FIX.
@@ -47,24 +53,25 @@ Section fn.
       pt_size := 1;
       pt_own (tr: (predₛ _ → predlₛ _)%ST) tid vl := tc_opaque
         (∃fb kb (bl: plistc _ _) e H, ⌜vl = [@RecV fb (kb :: bl) e H]⌝ ∗
-        ▷ □ ∀x ϝ k pre (wl: plistc _ _), typed_body (fp_E (fp x) ϝ) [ϝ ⊑ₗ []]
-          [k ◁cont{[ϝ ⊑ₗ []], λ v: vec _ 1, +[vhd v ◁ box (fp x).(fp_oty)] } pre]
-          (hzip_with (λ _ ty (v: val), v ◁ box ty) (fp x).(fp_ityl) wl)
-          (subst' fb (RecV fb (kb :: bl) e) $ subst' kb k $ subst'_pv bl wl e)
-          (tr (λ b: 𝔅, pre -[b])))
+        ▷ □ ∀x ϝ k ℭl (T: _ ℭl) pre (wl: plistc _ _),
+          typed_body (fp_E (fp x) ϝ) [ϝ ⊑ₗ []]
+            [k ◁cont{[ϝ ⊑ₗ []], λ v: vec _ 1, vhd v ◁ box (fp x).(fp_oty) +:: T} pre]
+            (hzip_with (λ _ ty (w: val), w ◁ box ty) (fp x).(fp_ityl) wl h++ T)
+            (subst' fb (RecV fb (kb :: bl) e) $ subst' kb k $ subst_plv bl wl e)
+            (λ acl, tr (λ b: 𝔅, pre (b -:: psepr acl)) (psepl acl)))
     |}%I.
   Next Obligation. rewrite /tc_opaque. apply _. Qed.
   Next Obligation. move=> *. by iDestruct 1 as (?????->) "?". Qed.
 
   Global Instance fn_ne n :
-    Proper (pointwise_relation A (fn_params_dist n) ==> dist n) fn.
+    Proper (pointwise_relation A (fn_params_dist n) ==> (≡{n}≡)) fn.
   Proof.
     move=> fp fp' Eq. apply ty_of_st_ne, st_of_pt_ne. split; [done|]=>/= ???.
-    do 5 apply bi.exist_ne=> ?. do 3 f_equiv. f_equiv=> x. (do 7 f_equiv)=> wl.
+    do 5 apply bi.exist_ne=> ?. do 3 f_equiv. f_equiv=> x. (do 11 f_equiv)=> wl.
     rewrite /typed_body. (do 3 f_equiv)=> vπl.
     do 6 f_equiv; [by eapply fp_E_ne|]. do 2 f_equiv; [|f_equiv].
-    - rewrite/= /cctx_elt_interp. do 5 f_equiv. case=>/= ?[].
-      do 4 f_equiv. rewrite /tctx_elt_interp. do 8 f_equiv. apply Eq.
+    - rewrite !cctx_interp_singleton /cctx_elt_interp. do 3 f_equiv.
+      case=>/= [??]. rewrite /tctx_elt_interp. do 12 f_equiv. apply Eq.
     - move: (Eq x)=> [_[+ _]]. rewrite {1}/dist.
       move: (fp x).(fp_ityl) (fp' x).(fp_ityl)=> ??. clear=> Eq.
       dependent induction Eq; [done|]. case wl=> ??. case vπl=> ??/=.
@@ -77,13 +84,13 @@ Arguments fn_params {_ _} _ _.
 
 Instance elctx_empty : Empty (lft → elctx) := λ _, [].
 
-Notation "fn< p >( E ; ity , .. , ity' ) → oty" :=
+Notation "fn< p > ( E ; ity , .. , ity' ) → oty" :=
   (fn (λ p, FP E%EL (ity%T +:: .. (+[ity'%T]) ..) oty%T))
   (at level 99, p pattern, oty at level 200, format
-    "fn< p >( E ;  ity ,  .. ,  ity' )  →  oty") : lrust_type_scope.
-Notation "fn< p >( E ) → oty" := (fn (λ p, FP E%EL +[] oty%T))
+    "fn< p > ( E ;  ity ,  .. ,  ity' )  →  oty") : lrust_type_scope.
+Notation "fn< p > ( E ) → oty" := (fn (λ p, FP E%EL +[] oty%T))
   (at level 99, p pattern, oty at level 200, format
-    "fn< p >( E )  →  oty") : lrust_type_scope.
+    "fn< p > ( E )  →  oty") : lrust_type_scope.
 Notation "fn( E ; ity , .. , ity' ) → oty" :=
   (fn (λ _: (), FP E%EL (ity%T +:: .. (+[ity'%T]) ..) oty%T))
   (at level 99, oty at level 200, format
@@ -113,7 +120,8 @@ Section typing.
         apply uPred_primitive.later_contractive. destruct n=>/=; [done|by apply Eq]. }
     move=>/= n ty ty' *. apply bi.exist_ne=> ?. apply bi.sep_ne; [done|].
     do 5 apply bi.exist_ne=> ?. f_equiv. f_contractive. (do 2 f_equiv)=> x.
-    (do 7 f_equiv)=> wl. rewrite /typed_body. (do 3 f_equiv)=> vπl.
+    (do 11 f_equiv)=> wl. rewrite /typed_body. (do 3 f_equiv)=> acπl.
+    move: (papp_ex acπl)=> [aπl[?->]]. move: (NeIT x)=> [ITl[->NeITl]].
     have EqBox: ∀𝔄 (T: _ → _ 𝔄), TypeNonExpansive T → ∀vπ d tid vl,
       (box (T ty)).(ty_own) vπ d tid vl ≡{n}≡ (box (T ty')).(ty_own) vπ d tid vl.
     { move=> ?? Ne. apply box_type_contr=> *.
@@ -122,7 +130,7 @@ Section typing.
       - apply type_lft_morph_elctx_interp_proper=>//. apply _.
       - apply dist_dist_later. by apply Ne.
       - apply dist_S. by apply Ne. }
-    move: (NeIT x)=> [ITl[->NeITl]]. do 5 f_equiv; [|do 3 f_equiv=>/=; f_equiv].
+    do 5 f_equiv; [|do 3 f_equiv; [|f_equiv]].
     - apply equiv_dist. rewrite /fp_E /= !elctx_interp_app.
       do 2 f_equiv; [|f_equiv; [|f_equiv]].
       + elim: NeITl; [done|]=> ????? _ ?. rewrite /tyl_E /= !elctx_interp_app.
@@ -133,9 +141,9 @@ Section typing.
       + apply type_lft_morph_elctx_interp_proper=>//. apply _.
       + rewrite !elctx_interp_ty_outlv_E. apply lft_incl_equiv_proper_r.
         by iApply type_lft_morph_lft_equiv_proper.
-    - rewrite /cctx_elt_interp. do 4 f_equiv. case=>/= ?[].
+    - rewrite !cctx_interp_singleton /cctx_elt_interp. do 3 f_equiv. case=>/= ??.
       do 4 f_equiv. rewrite /tctx_elt_interp. do 6 f_equiv. by apply EqBox.
-    - clear -NeITl EqBox. induction NeITl, wl, vπl; [done|]=>/=.
+    - clear -NeITl EqBox. induction NeITl, wl, aπl; [done|]=>/=.
       f_equiv; [|done]. rewrite /tctx_elt_interp. do 6 f_equiv. by apply EqBox.
   Qed.
 
@@ -177,26 +185,26 @@ Section typing.
     have Eq: (bl: list _) = bl' by rewrite plistc_renew_eq.
     iExists fb, kb, bl', e, (rew [λ bl₀, _ (_ :b: _ :b: bl₀ +b+ _) _] Eq in H).
     simpl_eq. iSplit; [done|]. iNext. rewrite /typed_body.
-    iIntros (x ϝ k pre wl') "!> % %aπl' LFT TIME PROPH UNIQ #Efp' Na L #C T Obs".
-    rewrite subst'_pv_renew. set wl := plistc_renew _ wl'.
+    iIntros (x ϝ ??? pre wl') "!> % %acπl LFT TIME PROPH UNIQ #Efp' Na L C T Obs".
+    move: (papp_ex acπl)=> [aπl[cπl->]]. rewrite subst_plv_renew. set wl := plistc_renew _ wl'.
     iDestruct ("Big" with "[$E $Efp']") as "(Efp & InIl & InO)".
-    iApply ("fn" $! _ _ _ (λ '-[b], pre -[g b]) _
-      _ (plist_map_with (λ _ _, (∘)) fl aπl') with
-      "LFT TIME PROPH UNIQ Efp Na L [] [T] [Obs]").
-    - iRevert "InO C". iClear "#". iIntros "#(_&_& InO &_) [#C _]".
-      iSplitL; [|done]. iIntros "!>" (?[vπ[]]) "Na L [(%&%&%& ⧖ & oty) _] Obs".
-      iApply ("C" $! _ -[_] with "Na L [⧖ oty] Obs"). iSplitL; [|done].
+    iApply ("fn" $! _ _ _ _ _ (λ '(b -:: cl), pre (g b -:: cl)) _
+      _ (plist_map_with (λ _ _, (∘)) fl aπl -++ cπl) with
+      "LFT TIME PROPH UNIQ Efp Na L [C] [T] [Obs]").
+    - rewrite !cctx_interp_singleton. iRevert "InO C". iClear "#".
+      iIntros "#(_&_& InO &_) C". iIntros (?[??]) "Na L /=[(%&%&%& ⧖ & oty) Tf] Obs".
+      iApply ("C" $! _ (_ -:: _) with "Na L [⧖ oty $Tf] Obs").
       iExists _, _. iSplitR; [done|]. iFrame "⧖". by iApply "InO".
     - iRevert "InIl T". iClear "#". iIntros "?". iStopProof. rewrite /wl.
       move: (fp x).(fp_ityl) (fp' x).(fp_ityl)=> tyl tyl'. clear.
-      move: 𝔄l 𝔄l' tyl tyl' fl ew wl' aπl'. fix FIX 1. case=> [|??]; case=>//=;
+      move: 𝔄l 𝔄l' tyl tyl' fl ew wl' aπl. fix FIX 1. case=> [|??]; case=>//=;
       dependent destruction tyl; dependent destruction tyl'; [by iIntros|].
       iIntros ([]?[][]) "/= #[(_&_& In &_) ?] [t ?]".
       iSplitL "t"; [|by iApply FIX]. iDestruct "t" as (???) "[⧖ ?]".
       iExists _, _. iSplit; [done|]. iFrame "⧖". by iApply "In".
-    - iApply proph_obs_eq; [|done]=>/= ?. f_equal. clear.
-      move: 𝔄l 𝔄l' fl aπl'. fix FIX 1. case=> [|??]; case=>//= ??[??][??].
-      f_equal. apply FIX.
+    - iApply proph_obs_eq; [|done]=>/= ?. rewrite !papply_app !papp_sepl !papp_sepr.
+      f_equal. clear. move: 𝔄l 𝔄l' fl aπl. fix FIX 1.
+      case=> [|??]; case=>//= ??[??][??]. f_equal. apply FIX.
   Qed.
 
   Lemma fn_subtype_specialize {A B 𝔄l 𝔅} (σ: A → B) (fp: _ → _ 𝔄l 𝔅) E L :
@@ -207,177 +215,114 @@ Section typing.
     iIntros "Big" (?). iApply "Big".
   Qed.
 
-(*
-  (* In principle, proving this hard-coded to an empty L would be sufficient --
-     but then we would have to require elctx_sat as an Iris assumption. *)
-  Lemma type_call_iris' E L (κs : list lft) {A} x (ps : list path) qκs qL tid
-        p (k : expr) (fp : A → fn_params (length ps)) :
-    (∀ ϝ, elctx_sat (((λ κ, ϝ ⊑ₑ κ) <$> κs) ++ E) L (fp_E (fp x) ϝ)) →
-    AsVal k →
-    lft_ctx -∗ time_ctx -∗ elctx_interp E -∗ na_own tid ⊤ -∗ llctx_interp L qL -∗
-    qκs.[lft_intersect_list κs] -∗
-    tctx_elt_interp tid (p ◁ fn fp) -∗
-    ([∗ list] y ∈ zip_with TCtx_hasty ps (box <$> vec_to_list (fp x).(fp_ityl)),
-                   tctx_elt_interp tid y) -∗
-    (∀ ret depth,
-        na_own tid ⊤ -∗ llctx_interp L qL -∗ qκs.[lft_intersect_list κs] -∗
-        ⧖depth -∗ (box (fp x).(fp_oty)).(ty_own) depth tid [ret] -∗
-        WP k [of_val ret] {{ _, cont_postcondition }}) -∗
-    WP (call: p ps → k) {{ _, cont_postcondition }}.
+  Local Lemma wp_app_hasty_box {𝔄l} vl r (f: val)
+    (pl: plistc _ 𝔄l) tyl vπl tid (Φ: val → iProp Σ) :
+    tctx_interp tid (hzip_with (λ _ ty q, q ◁ box ty) tyl pl) vπl -∗
+    (∀wl: plistc _ _,
+      tctx_interp tid (hzip_with (λ _ ty (w: val), w ◁ box ty) tyl wl) vπl -∗
+      WP f (of_val r :: map of_val (vl ++ wl)) {{ Φ }}) -∗
+    WP f (of_val r :: map of_val vl ++ pl) {{ Φ }}.
   Proof.
-    iIntros (HE [k' <-]) "#LFT #TIME #HE Htl HL Hκs Hf Hargs Hk".
-    wp_apply (wp_hasty with "Hf"). iIntros (depth v) "Hdepth % Hf".
-    iApply (wp_app_vec _ _ (_::_) ((λ v, ⌜v = (λ: ["_r"], (#☠ ;; #☠) ;; k' ["_r"])%V⌝):::
-               vmap (λ ty (v : val), tctx_elt_interp tid (v ◁ box ty)) (fp x).(fp_ityl))%I
-            with "[Hargs]").
-    - rewrite /=. iSplitR "Hargs".
-      { simpl. iApply wp_value. by unlock. }
-      remember (fp_ityl (fp x)) as tys. clear dependent k' p HE fp x.
-      iInduction ps as [|p ps] "IH" forall (tys); first by simpl.
-      simpl in tys. inv_vec tys=>ty tys. simpl.
-      iDestruct "Hargs" as "[HT Hargs]". iSplitL "HT".
-      + iApply (wp_hasty with "HT"). iIntros (??) "???".
-        rewrite tctx_hasty_val. auto.
-      + iApply "IH". done.
-    - simpl. change (@length expr ps) with (length ps).
-      iIntros (vl'). inv_vec vl'=>kv vl; csimpl.
-      iIntros "[-> Hvl]". iDestruct "Hf" as (fb kb xb e ?) "[EQ [EQl #Hf]]".
-      iDestruct "EQ" as %[=->]. iDestruct "EQl" as %EQl.
-      revert vl fp HE. rewrite /= -EQl=>vl fp HE. wp_rec.
-      iMod (lft_create with "LFT") as (ϝ) "[Htk #Hinh]"; first done.
-      iSpecialize ("Hf" $! x ϝ _ vl). iDestruct (HE ϝ with "HL") as "#HE'".
-      iMod (bor_create _ ϝ with "LFT Hκs") as "[Hκs HκsI]"; first done.
-      iDestruct (frac_bor_lft_incl with "LFT [>Hκs]") as "#Hκs".
-      { iApply (bor_fracture with "LFT"); first done. by rewrite Qp_mul_1_r. }
-      iApply ("Hf" with "LFT TIME [] Htl [Htk] [Hk HκsI HL]").
-      + iApply "HE'". iIntros "{$# Hf Hinh HE' LFT TIME HE %}".
-        iInduction κs as [|κ κs] "IH"=> //=. iSplitL.
-        { iApply lft_incl_trans; first done. iApply lft_intersect_incl_l. }
-        iApply "IH". iModIntro. iApply lft_incl_trans; first done.
-        iApply lft_intersect_incl_r.
-      + iSplitL; last done. iExists ϝ. iSplit; first by rewrite /= left_id.
-        iFrame "#∗".
-      + iIntros (y) "IN". iDestruct "IN" as %->%elem_of_list_singleton.
-        iIntros (args) "Htl [Hϝ _] [Hret _]". inv_vec args=>r.
-        iDestruct "Hϝ" as  (κ') "(EQ & Htk & _)". iDestruct "EQ" as %EQ.
-        rewrite /= left_id in EQ. subst κ'. simpl. wp_rec. wp_bind Endlft.
-        iSpecialize ("Hinh" with "Htk"). iClear "Hκs".
-        iApply (wp_mask_mono _ (↑lftN ∪ ↑lft_userN)); first done.
-        iApply (wp_step_fupd with "Hinh"); [set_solver-..|]. wp_seq.
-        iIntros "#Htok !>". wp_seq. iMod ("HκsI" with "Htok") as ">Hκs".
-        rewrite tctx_hasty_val. iDestruct "Hret" as (?) "[#? Hret]".
-        by iApply ("Hk" with "Htl HL Hκs").
-      + rewrite /tctx_interp vec_to_list_map !zip_with_fmap_r
-                (zip_with_zip (λ v ty, (v, _))) zip_with_zip !big_sepL_fmap.
-        iApply (big_sepL_mono' with "Hvl"); last done. by iIntros (i [v ty']).
+    move: tyl pl vπl vl. elim 𝔄l=> [|?? IH]; dependent destruction tyl.
+    { iIntros "* _ Wp". iSpecialize ("Wp" $! -[] with "[//]"). by rewrite !right_id. }
+    iIntros ([p pl'][??]vl) "/= [p pl'] ToWp".
+    have ->: App f (of_val r :: map of_val vl ++ p :: pl') =
+      fill_item (AppRCtx f (r :: vl) pl') p by done.
+    iApply wp_bind. iApply (wp_hasty with "p"). iIntros (w ? _) "⧖ p".
+    have ->: fill_item (AppRCtx f (r :: vl) pl') w =
+      App f (of_val r :: map of_val (vl ++ [w]) ++ pl') by rewrite map_app -assoc.
+    iApply (IH with "pl'"). iIntros (?) "pl'". rewrite -assoc.
+    iApply ("ToWp" $! (_ -:: _)). iFrame "pl'". iExists w, _. iFrame "⧖ p".
+    by rewrite eval_path_of_val.
   Qed.
 
-  Lemma type_call_iris E (κs : list lft) {A} x (ps : list path) qκs tid
-        f (k : expr) (fp : A → fn_params (length ps)) :
-    (∀ ϝ, elctx_sat (((λ κ, ϝ ⊑ₑ κ) <$> κs) ++ E) [] (fp_E (fp x) ϝ)) →
-    AsVal k →
-    lft_ctx -∗ time_ctx -∗ elctx_interp E -∗ na_own tid ⊤ -∗
-    qκs.[lft_intersect_list κs] -∗
-    (fn fp).(ty_own) 0 tid [f] -∗
-    ([∗ list] y ∈ zip_with TCtx_hasty ps (box <$> vec_to_list (fp x).(fp_ityl)),
-                   tctx_elt_interp tid y) -∗
-    (∀ ret depth, na_own tid ⊤ -∗ qκs.[lft_intersect_list κs] -∗
-             ⧖depth -∗ (box (fp x).(fp_oty)).(ty_own) depth tid [ret] -∗
-             WP k [of_val ret] {{ _, cont_postcondition }}) -∗
-    WP (call: f ps → k) {{ _, cont_postcondition }}.
+  Lemma type_call {A 𝔄l 𝔅 ℭl 𝔇l 𝔈l} x (fp: A → _ 𝔄l 𝔅) p (ql: list _)
+    (ql': plistc _ _) (T: _ ℭl) (T': _ 𝔇l) tr k (Tk: _ → _ 𝔈l) pre tr' E L C :
+    ql = ql' → Forall (lctx_lft_alive E L) L.*1 →
+    (∀ϝ, elctx_sat (map (λ κ, ϝ ⊑ₑ κ) L.*1 ++ E) L (fp_E (fp x) ϝ)) →
+    tctx_extract_ctx E L (p ◁ fn fp +::
+      hzip_with (λ _ ty q, q ◁ box ty) (fp x).(fp_ityl) ql') T T' tr →
+    k ◁cont{L, Tk} pre ∈ C →
+    (∀ret: val, tctx_incl E L (ret ◁ box (fp x).(fp_oty) +:: T') (Tk [#ret]) tr') →
+    ⊢ typed_body E L C T (call: p ql → k) (tr (λ '(trp -:: adl),
+        let '(al, dl) := psep adl in trp (λ b: 𝔅, tr' pre (b -:: dl)) al))%type.
   Proof.
-    iIntros (HE Hk') "#LFT #TIME #HE Htl Hκs Hf Hargs Hk".
-    iMod persist_time_rcpt_0 as "#?".
-    iApply (type_call_iris' with "LFT TIME HE Htl [] Hκs [Hf] Hargs [Hk]"); [done|..].
-    - instantiate (1 := 1%Qp). by rewrite /llctx_interp.
-    - rewrite tctx_hasty_val. auto.
-    - iIntros "* Htl _". iApply "Hk". done.
+    iIntros (-> Alv ToEfp ?? InTk). iApply typed_body_tctx_incl; [done|].
+    iIntros (?[? adπl]). move: (papp_ex adπl)=> [aπl[dπl->]].
+    iIntros "/= #LFT #TIME #PROPH #UNIQ #E Na L C [p[ql T']] Obs".
+    iMod (lctx_lft_alive_tok_list with "E L") as (?) "(κL & L & ToL)"; [done|done|].
+    iMod (lft_create with "LFT") as (ϝ) "[ϝ #To†ϝ]"; [done|].
+    iMod (bor_create _ ϝ with "LFT κL") as "[BorκL ToκL]"; [done|].
+    iDestruct (frac_bor_lft_incl with "LFT [>BorκL]") as "#?".
+    { iApply (bor_fracture with "LFT"); [done|]. by rewrite Qp_mul_1_r. }
+    iDestruct (ToEfp ϝ with "L [$E]") as "#Efp".
+    { move: L.*1=> κl. iInduction κl as [|κ κl] "IH"; [done|]=>/=.
+      iSplit. { iApply lft_incl_trans; [done|]. iApply lft_intersect_incl_l. }
+      iApply "IH". iModIntro. iApply lft_incl_trans; [done|].
+      iApply lft_intersect_incl_r. }
+    rewrite /call_def. wp_apply (wp_hasty with "p"). iIntros (???) "_".
+    iDestruct 1 as (trp->?????[=->]) "Body".
+    have ->: (λ: ["_r"], Skip;; k ["_r"])%E = (λ: ["_r"], Skip;; k ["_r"])%V by unlock.
+    iApply (wp_app_hasty_box [] with "ql")=>/=. iIntros (?) "ityl". wp_rec.
+    iApply ("Body" with "LFT TIME PROPH UNIQ Efp Na [ϝ] [C ToκL L ToL]
+      [ityl T'] Obs"); first 2 last.
+    { rewrite big_sepHL_1_app. iFrame. } { iSplitL; [|done]. iExists _.
+    iSplit; [by rewrite/= left_id|]. by iFrame "ϝ". }
+    rewrite cctx_interp_singleton. iIntros (v[bπ ?]). inv_vec v=> v.
+    iIntros "Na [(%& %Eq & ϝ &_) _] [oty Tk] Obs". rewrite/= left_id in Eq.
+    rewrite -Eq. wp_rec. wp_bind Skip. iSpecialize ("To†ϝ" with "ϝ").
+    iApply (wp_mask_mono _ (↑lftN ∪ ↑lft_userN)); [done|].
+    iApply (wp_step_fupd with "To†ϝ"); [set_solver|]. wp_seq. iIntros "†ϝ !>".
+    wp_seq. iMod ("ToκL" with "†ϝ") as "> κL". iMod ("ToL" with "κL L") as "L".
+    iSpecialize ("C" with "[//]"). have ->: [v: expr] = map of_val ([#v]) by done.
+    iMod (InTk _ _ _ (_ -:: _) with "LFT PROPH UNIQ E L [$oty $Tk] Obs")
+    as (?) "(L & Tk & Obs)". iApply ("C" with "Na L Tk Obs").
   Qed.
 
-  Lemma type_call' E L (κs : list lft) T p (ps : list path)
-                   {A} (fp : A → fn_params (length ps)) (k : val) x :
-    Forall (lctx_lft_alive E L) κs →
-    (∀ ϝ, elctx_sat (((λ κ, ϝ ⊑ₑ κ) <$> κs) ++ E) L (fp_E (fp x) ϝ)) →
-    ⊢ typed_body E L [k ◁cont(L, λ v : vec _ 1, ((v!!!0%fin:val) ◁ box (fp x).(fp_oty)) :: T)]
-               ((p ◁ fn fp) ::
-                zip_with TCtx_hasty ps (box <$> vec_to_list (fp x).(fp_ityl)) ++
-                T)
-               (call: p ps → k).
+  Lemma type_letcall {A 𝔄l 𝔅 ℭl 𝔇l} x (fp: A → _ 𝔄l 𝔅) p (ql: list _)
+    (ql': plistc _ _) (T: _ ℭl) (T': _ 𝔇l) b e tr pre E L C :
+    ql = ql' → Closed (b :b: []) e → Closed [] p → Forall (Closed []) ql →
+    Forall (lctx_lft_alive E L) L.*1 →
+    (∀ϝ, elctx_sat (map (λ κ, ϝ ⊑ₑ κ) L.*1 ++ E) L (fp_E (fp x) ϝ)) →
+    tctx_extract_ctx E L (p ◁ fn fp +::
+      hzip_with (λ _ ty q, q ◁ box ty) (fp x).(fp_ityl) ql') T T' tr →
+    (∀ret: val, typed_body E L C
+      (ret ◁ box (fp x).(fp_oty) +:: T') (subst' b ret e) pre) -∗
+    typed_body E L C T (letcall: b := p ql in e) (tr (λ '(trp -:: adl),
+      let '(al, dl) := psep adl in trp (λ b: 𝔅, pre (b -:: dl)) al)).
   Proof.
-    iIntros (Hκs HE tid) "#LFT #TIME #HE Htl HL HC (Hf & Hargs & HT)".
-    iMod (lctx_lft_alive_tok_list _ _ κs with "HE HL") as (q) "(Hκs & HL & Hclose)"; [done..|].
-    iApply (type_call_iris' with "LFT TIME HE Htl HL Hκs Hf Hargs"); [done|].
-    iIntros (r depth) "Htl HL Hκs Hdepth Hret". iMod ("Hclose" with "Hκs HL") as "HL".
-    iSpecialize ("HC" with "[]"); first by (iPureIntro; apply elem_of_list_singleton).
-    iApply ("HC" $! [#r] with "Htl HL").
-    rewrite tctx_interp_cons tctx_hasty_val. auto with iFrame.
-  Qed.
-
-  (* Specialized type_call':  Adapted for use by solve_typing; fixed "list of
-     alive lifetimes" to be the local ones. *)
-  Lemma type_call {A} x E L C T T' T'' p (ps : list path)
-                        (fp : A → fn_params (length ps)) k :
-    p ◁ fn fp ∈ T →
-    Forall (lctx_lft_alive E L) (L.*1) →
-    (∀ ϝ, elctx_sat (((λ κ, ϝ ⊑ₑ κ) <$> (L.*1)) ++ E) L (fp_E (fp x) ϝ)) →
-    tctx_extract E L (zip_with TCtx_hasty ps
-                                   (box <$> vec_to_list (fp x).(fp_ityl))) T T' →
-    k ◁cont(L, T'') ∈ C →
-    (∀ ret : val, tctx_incl E L ((ret ◁ box (fp x).(fp_oty))::T') (T'' [# ret])) →
-    ⊢ typed_body E L C T (call: p ps → k).
-  Proof.
-    intros Hfn HL HE HTT' HC HT'T''.
-    rewrite -typed_body_mono /flip; last done; first by eapply type_call'.
-    - etrans. eapply (incl_cctx_incl _ [_]); first by intros ? ->%elem_of_list_singleton.
-      apply cctx_incl_cons; first done. intros args. by inv_vec args.
-    - etrans; last by apply (tctx_incl_frame_l [_]).
-      apply copy_elem_of_tctx_incl; last done. apply _.
-  Qed.
-
-  Lemma type_letcall {A} x E L C T T' p (ps : list path)
-                        (fp : A → fn_params (length ps)) b e :
-    Closed (b :b: []) e → Closed [] p → Forall (Closed []) ps →
-    p ◁ fn fp ∈ T →
-    Forall (lctx_lft_alive E L) (L.*1) →
-    (∀ ϝ, elctx_sat (((λ κ, ϝ ⊑ₑ κ) <$> (L.*1)) ++ E) L (fp_E (fp x) ϝ)) →
-    tctx_extract E L (zip_with TCtx_hasty ps
-                                   (box <$> vec_to_list (fp x).(fp_ityl))) T T' →
-    (∀ ret : val, typed_body E L C ((ret ◁ box (fp x).(fp_oty))::T') (subst' b ret e)) -∗
-    typed_body E L C T (letcall: b := p ps in e).
-  Proof.
-    iIntros (?? Hpsc ????) "He".
-    iApply (type_cont_norec [_] _ (λ r, ((r!!!0%fin:val) ◁ box (fp x).(fp_oty)) :: T')).
+    iIntros (->?? Clql ???) "e". iApply type_cont_norec.
     - (* TODO : make [solve_closed] work here. *)
-      eapply is_closed_weaken; first done. set_solver+.
+      eapply is_closed_weaken; [done|]. set_solver+.
     - (* TODO : make [solve_closed] work here. *)
       rewrite /Closed /= !andb_True. split.
       + by eapply is_closed_weaken, list_subseteq_nil.
-      + eapply Is_true_eq_left, forallb_forall, List.Forall_forall, Forall_impl=>//.
-        intros. eapply Is_true_eq_true, is_closed_weaken=>//. set_solver+.
+      + eapply Is_true_eq_left, forallb_forall, List.Forall_forall, Forall_impl
+        =>// ??. eapply Is_true_eq_true, is_closed_weaken=>//. set_solver+.
     - iIntros (k).
       (* TODO : make [simpl_subst] work here. *)
-      change (subst' "_k" k (p ((λ: ["_r"], (#☠ ;; #☠) ;; "_k" ["_r"])%E :: ps))) with
-             ((subst "_k" k p) ((λ: ["_r"], (#☠ ;; #☠) ;; k ["_r"])%E :: map (subst "_k" k) ps)).
-      rewrite is_closed_nil_subst //.
-      assert (map (subst "_k" k) ps = ps) as ->.
-      { clear -Hpsc. induction Hpsc=>//=. rewrite is_closed_nil_subst //. congruence. }
-      iApply type_call; try done. constructor. done.
-    - simpl. iIntros (k ret). inv_vec ret=>ret. rewrite /subst_v /=.
-      rewrite ->(is_closed_subst []); last set_solver+; last first.
-      { apply subst'_is_closed; last done. apply is_closed_of_val. }
-      (iApply typed_body_mono; last by iApply "He"); [|done..].
-      apply incl_cctx_incl. set_solver+.
+      have ->: subst' "_k" k (call: p ql' → "_k")%E = subst "_k" k p $
+        (λ: ["_r"], Skip;; k ["_r"])%E :: map (subst "_k" k) ql' by done.
+      rewrite is_closed_nil_subst; [|done].
+      have ->: map (subst "_k" k) ql' = ql'.
+      { clear -Clql. elim Clql; [done|]=>/= ????->. by rewrite is_closed_nil_subst. }
+      iApply typed_body_eq; last first. { iApply type_call=>//; [constructor|]=> v.
+      have {1}->: v = vhd [#v] by done. move: [#v]=> ?. apply tctx_incl_refl. } done.
+    - iIntros (k ret). inv_vec ret=>ret. rewrite /subst_v /=.
+      rewrite (is_closed_subst []); [| |set_solver+]; last first.
+      { apply subst'_is_closed; [|done]. apply is_closed_of_val. } iApply "e".
   Qed.
-*)
 
-  Lemma type_fnrec_instr {A 𝔄l 𝔅} (tr: (predₛ 𝔅 → predlₛ 𝔄l)%ST) (fp: A → _)
+  Lemma type_fnrec_instr {A 𝔄l 𝔅} (tr: pred' 𝔅 → predl 𝔄l) (fp: A → _)
     fb (bl: plistc _ _) e E L :
     Closed (fb :b: "return" :: bl +b+ []) e →
-    □ (∀x ϝ (f: val) k pre (wl: plistc _ 𝔄l), typed_body (fp_E (fp x) ϝ) [ϝ ⊑ₗ []]
-      [k ◁cont{[ϝ ⊑ₗ []], λ v: vec _ 1, +[vhd v ◁ box (fp x).(fp_oty)] } pre]
-      (f ◁ fn fp +:: hzip_with (λ _ ty (v: val), v ◁ box ty) (fp x).(fp_ityl) wl)
-      (subst' fb f $ subst "return" k $ subst'_pv bl wl e)
-      (λ '(tr' -:: al), tr' = tr ∧ tr (λ b: 𝔅, pre -[b]) al)%type) -∗
+    □ (∀x ϝ (f: val) k ℭl (T: _ ℭl) pre (wl: plistc _ 𝔄l),
+      typed_body (fp_E (fp x) ϝ) [ϝ ⊑ₗ []]
+        [k ◁cont{[ϝ ⊑ₗ []], λ v: vec _ 1, vhd v ◁ box (fp x).(fp_oty) +:: T} pre]
+        (f ◁ fn fp +:: hzip_with (λ _ ty (v: val), v ◁ box ty) (fp x).(fp_ityl) wl h++ T)
+        (subst' fb f $ subst "return" k $ subst_plv bl wl e)
+        (λ '(tr' -:: acl), tr' = tr ∧ let '(al, cl) := psep acl in
+          tr (λ b: 𝔅, pre (b -:: cl)) al)%type) -∗
     typed_instr_ty E L +[] (fnrec: fb bl := e) (fn fp) (λ post _, post tr).
   Proof.
     iIntros (Cl) "#Body %%% _ _ _ _ _ $$ _ Obs". iMod persist_time_rcpt_0 as "#⧖".
@@ -386,18 +331,20 @@ Section typing.
     iSplit; [|done]. iLöb as "IH". iExists _, 0. iSplit; [by rewrite/= decide_left|].
     iFrame "⧖". iExists tr=>/=. iSplit; [done|]. iExists fb, "return", bl, e, _.
     iSplit; [done|]. iIntros "!>!> * %% LFT TIME PROPH UNIQ Efp Na L C T ?".
-    iApply ("Body" $! _ _ (RecV _ _ _) _ _ _ _ (_ -:: _) with
+    iApply ("Body" $! _ _ (RecV _ _ _) _ _ _ _ _ _ (_ -:: _) with
       "LFT TIME PROPH UNIQ Efp Na L C [$T $IH]").
     by iApply proph_obs_impl; [|done]=>/= ??.
   Qed.
 
-  Lemma type_fn_instr {A 𝔄l 𝔅} (tr: (predₛ 𝔅 → predlₛ 𝔄l)%ST) (fp: A → _)
+  Lemma type_fn_instr {A 𝔄l 𝔅} (tr: pred' 𝔅 → predl 𝔄l) (fp: A → _)
     (bl: plistc _ _) e E L :
     Closed ("return" :: bl +b+ []) e →
-    □ (∀x ϝ k pre (wl: plistc _ _), typed_body (fp_E (fp x) ϝ) [ϝ ⊑ₗ []]
-      [k ◁cont{[ϝ ⊑ₗ []], λ v: vec _ 1, +[vhd v ◁ box (fp x).(fp_oty)] } pre]
-      (hzip_with (λ _ ty (v: val), v ◁ box ty) (fp x).(fp_ityl) wl)
-      (subst "return" k $ subst'_pv bl wl e) (tr (λ b: 𝔅, pre -[b]))) -∗
+    □ (∀x ϝ k ℭl (T: _ ℭl) pre (wl: plistc _ 𝔄l),
+      typed_body (fp_E (fp x) ϝ) [ϝ ⊑ₗ []]
+        [k ◁cont{[ϝ ⊑ₗ []], λ v: vec _ 1, vhd v ◁ box (fp x).(fp_oty) +:: T} pre]
+        (hzip_with (λ _ ty (v: val), v ◁ box ty) (fp x).(fp_ityl) wl h++ T)
+        (subst "return" k $ subst_plv bl wl e)
+        (λ acl, let '(al, cl) := psep acl in tr (λ b: 𝔅, pre (b -:: cl)) al)%type) -∗
     typed_instr_ty E L +[] (fn: bl := e) (fn fp) (λ post _, post tr).
   Proof.
     iIntros (?) "#?". iApply type_fnrec_instr. iIntros "!> *".
