theories/typing/cont.v
@@ -7,29 +7,44 @@ Section typing.
   Context `{!typeG Σ}.
 
   (** Jumping to and defining a continuation. *)
-  Lemma type_jump {𝔄l 𝔅l} E (T: _ 𝔄l) C k L n (T': _ → _ 𝔅l) pre vl (vl': vec _ n) tr :
-    k ◁cont{L, T'} pre ∈ C →
-    vl = map of_val vl' → tctx_incl E L T (T' vl') tr →
-    ⊢ typed_body E L C T (k vl) (tr pre).
+  Lemma type_jump {𝔄l 𝔅l} E (T: _ 𝔄l) C k L n (T': _ → _ 𝔅l) pre el (vl: vec _ n) tr :
+    k ◁cont{L, T'} pre ∈ C → el = map of_val vl → tctx_incl E L T (T' vl) tr →
+    ⊢ typed_body E L C T (k el) (tr pre).
   Proof.
     iIntros (InC -> TT' ??) "LFT _ PROPH UNIQ E Na L C T Obs".
     iMod (TT' with "LFT PROPH UNIQ E L T Obs") as (?) "(L & T & Obs)".
-    rewrite cctx_interp_forall. iSpecialize ("C" with "[%//]").
-    iApply ("C" with "Na L T Obs").
+    iSpecialize ("C" with "[%//]"). iApply ("C" with "Na L T Obs").
   Qed.
 
-  Lemma type_cont {𝔄l 𝔅l} E L C (T: tctx 𝔄l) kb bl ec e L' (T': _ → _ 𝔅l) prec pre :
+  Lemma type_cont {𝔄l 𝔅l} E L C (T: _ 𝔄l) kb bl ec e L' (T': _ → _ 𝔅l) prek pre :
     Closed (kb :b: bl +b+ []) ec → Closed (kb :b: []) e →
-    (∀k, typed_body E L (k ◁cont{L', T'} prec :: C) T (subst' kb k e) pre) -∗
-    □(∀k (vl: vec val (length bl)), typed_body E L' (k ◁cont{L', T'} prec :: C)
-        (T' vl) (subst_v (kb :: bl) (k ::: vl) ec) prec) -∗
+    (∀k, typed_body E L (k ◁cont{L', T'} prek :: C) T (subst' kb k e) pre) -∗
+    □(∀k (vl: vec val (length bl)), typed_body E L' (k ◁cont{L', T'} prek :: C)
+      (T' vl) (subst' kb k $ subst_v bl vl ec) prek) -∗
     typed_body E L C T (letcont: kb bl := ec in e) pre.
   Proof.
-    iIntros (??) "e #ec". iIntros (??) "#LFT #TIME #PROPH #UNIQ #E Na L #C T Obs".
-    rewrite (_ : (rec: kb bl := ec)%E = of_val (rec: kb bl := ec)%V); [|by unlock].
-    wp_let. iApply ("e" with "LFT TIME PROPH UNIQ E Na L [$C] T Obs").
-    iLöb as "IH". iIntros "!>" (??) "Na L' T' Obs". wp_rec.
-    by iApply ("ec" with "LFT TIME PROPH UNIQ E Na L' [$C] T' Obs").
+    iIntros (??) "e #ec". iIntros (??) "#LFT #TIME #PROPH #UNIQ #E Na L C T Obs".
+    have ->: (rec: kb bl := ec)%E = of_val (rec: kb bl := ec) by unlock.
+    wp_let. iApply ("e" with "LFT TIME PROPH UNIQ E Na L [C] T Obs").
+    iLöb as "IH". iIntros (?). rewrite elem_of_cons.
+    iIntros ([->|?]); [|by iApply "C"]. iIntros (??) "Na L' T' Obs".
+    wp_rec. iApply ("ec" with "LFT TIME PROPH UNIQ E Na L' [C] T' Obs").
+    by iApply "IH".
+  Qed.
+
+  Lemma type_cont_norec {𝔄l 𝔅l} E L C (T: _ 𝔄l) kb bl ec e L' (T': _ → _ 𝔅l) prek pre :
+    Closed (kb :b: bl +b+ []) ec → Closed (kb :b: []) e →
+    (∀k, typed_body E L (k ◁cont{L', T'} prek :: C) T (subst' kb k e) pre) -∗
+    (∀k (vl: vec val (length bl)),
+      typed_body E L' C (T' vl) (subst' kb k $ subst_v bl vl ec) prek) -∗
+    typed_body E L C T (letcont: kb bl := ec in e) pre.
+  Proof.
+    iIntros (??) "e ec". iIntros (??) "#LFT #TIME #PROPH #UNIQ #E Na L C T Obs".
+    have ->: (rec: kb bl := ec)%E = of_val (rec: kb bl := ec) by unlock.
+    wp_let. iApply ("e" with "LFT TIME PROPH UNIQ E Na L [ec C] T Obs").
+    iIntros (?). rewrite elem_of_cons.
+    iIntros ([->|?]); [|by iApply "C"]. iIntros (??) "Na L' T' Obs".
+    wp_rec. by iApply ("ec" with "LFT TIME PROPH UNIQ E Na L' [C] T' Obs").
   Qed.
 
 End typing.
